Clean/Circuit.lean
@@ -4,6 +4,7 @@ import Clean.Circuit.LookupCircuit
 import Clean.Circuit.Explicit
 import Clean.Circuit.Extensions
 import Clean.Circuit.StructEvalSimprocs
+import Clean.Circuit.Verifier
 import Clean.Utils.Tactics.ProvableStructDeriving
 import Clean.Gadgets.Equality
 import Clean.Gadgets.Conditional
